Streamline syntactic equivalence checker proofs.

SmtEquivChecker.v
@@ -21,10 +21,10 @@ Fixpoint symbolize_expr (e : expr) : smt_expr :=
 Parameter sym_checker :  smt_expr -> smt_expr -> bool.
 
 (* Soundness of Z3: if the symbolic versions of 2 exprs are shown equivalent by z3, then the 2 exprs are equivalent *)
-Axiom sound_sym_checker : forall e1 e2 : expr, sym_checker (symbolize_expr e1) (symbolize_expr e2) = true -> forall s, aequiv e1 e2 s.
+Axiom sound_smt_checker : forall e1 e2 : expr, sym_checker (symbolize_expr e1) (symbolize_expr e2) = true -> forall s, aequiv e1 e2 s.
 
 (* And prove it equivalent in the same way ... *)
-Definition smt_equivalence_checker (e1 e2 : expr) (s : state) : bool := 
+Definition smt_equiv_checker (e1 e2 : expr) (s : state) : bool := 
   match e1, e2 with
     | Constant n1, Constant n2 => Nat.eqb n1 n2
     | Var name1, Var name2 => String.eqb name1 name2
