Main.v
@@ -2,11 +2,11 @@ Require Import Arith.
 Require Import Bool.
 From Coq Require Import Strings.String.
 Open Scope string_scope.
-From MyProject Require Export EquivalenceChecker.
-From MyProject Require Export SmtEquivalenceChecker.
+From MyProject Require Export SynEquivChecker.
+From MyProject Require Export SmtEquivChecker.
 
-Lemma one_more_lemma (e1 e2 : expr)  (s : state) :
-  equivalence_checker e1 e2 s = true -> e1 = e2.
+Lemma sound_syn_checker (e1 e2 : expr)  (s : state) :
+  syn_equiv_checker e1 e2 s = true -> e1 = e2.
   Proof.
     intros H.
     revert H.
@@ -38,77 +38,15 @@ Lemma one_more_lemma (e1 e2 : expr)  (s : state) :
       reflexivity.
   Qed.
 
-Lemma plus_lemma: (forall (e1_1 e1_2 e2_1 e2_2 : expr) (s : state), 
-  equivalence_checker e1_1 e2_1 s &&
-  equivalence_checker e1_2 e2_2 s = true -> Plus e1_1 e1_2 = Plus e2_1 e2_2).
-  Proof.
-    intros.
-    apply Bool.andb_true_iff in H.
-    destruct H.
-    apply one_more_lemma in H.
-    apply one_more_lemma in H0.
-    rewrite H.
-    rewrite H0.
-    reflexivity.
-Qed.
-
-Lemma minus_lemma: (forall (e1_1 e1_2 e2_1 e2_2 : expr) (s : state), 
-  equivalence_checker e1_1 e2_1 s &&
-  equivalence_checker e1_2 e2_2 s = true -> Minus e1_1 e1_2 = Minus e2_1 e2_2).
-  Proof.
-    intros.
-    apply Bool.andb_true_iff in H.
-    destruct H.
-    apply one_more_lemma in H.
-    apply one_more_lemma in H0.
-    rewrite H.
-    rewrite H0.
-    reflexivity.
-Qed.
-
-
-Lemma mul_lemma: (forall (e1_1 e1_2 e2_1 e2_2 : expr) (s : state), 
-  equivalence_checker e1_1 e2_1 s &&
-  equivalence_checker e1_2 e2_2 s = true -> Mul e1_1 e1_2 = Mul e2_1 e2_2).
-  Proof.
-    intros.
-    apply Bool.andb_true_iff in H.
-    destruct H.
-    apply one_more_lemma in H.
-    apply one_more_lemma in H0.
-    rewrite H.
-    rewrite H0.
-    reflexivity.
-Qed.
-
-Lemma lemma1 :
-  forall (e1 e2 : expr) (s : state), equivalence_checker e1 e2 s = true -> e1 = e2.
-  Proof.
-    intros e1 e2 s.
-    unfold equivalence_checker.
-    destruct e1, e2; try discriminate.
-    - intros H.
-      apply Nat.eqb_eq in H.
-      rewrite H.
-      reflexivity.
-    - apply plus_lemma.
-    - apply minus_lemma.
-    - apply mul_lemma.
-    - intros H.
-      apply String.eqb_eq in H.
-      rewrite H.
-      reflexivity.
-Qed.
-
 (* Prove that the equivalence checker is correct *)
-Theorem equivalence_checker_correct:
-  forall (e1 e2 : expr) (s : state), equivalence_checker e1 e2 s = true -> aequiv e1 e2 s.
+Theorem syn_equiv_checker_correct:
+  forall (e1 e2 : expr) (s : state), syn_equiv_checker e1 e2 s = true -> aequiv e1 e2 s.
 Proof.
 intros e1 e2.
 unfold aequiv.
 intros s.
 intros H.
-apply lemma1 in H.
+apply sound_syn_checker in H.
 rewrite H.
 reflexivity.
 Qed.
@@ -130,28 +68,28 @@ Lemma smt_plus_lemma:
  Qed.
 
 (* Prove that the SMT equivalence checker is correct *)
-Theorem smt_equivalence_checker_correct:
-  forall (e1 e2 : expr) (s : state), smt_equivalence_checker e1 e2 s = true -> aequiv e1 e2 s.
+Theorem smt_equiv_checker_correct:
+  forall (e1 e2 : expr) (s : state), smt_equiv_checker e1 e2 s = true -> aequiv e1 e2 s.
 Proof.
   intros e1 e2 s.
   unfold aequiv.
   intros H.
   destruct e1, e2; try discriminate.
-  - unfold smt_equivalence_checker in H.
+  - unfold smt_equiv_checker in H.
     apply Nat.eqb_eq in H.
     rewrite H.
     reflexivity.
-  - unfold smt_equivalence_checker in H.
-    apply sound_sym_checker.
+  - unfold smt_equiv_checker in H.
+    apply sound_smt_checker.
     rewrite smt_plus_lemma.
     rewrite smt_plus_lemma.
     apply H.
-  - unfold smt_equivalence_checker in H.
-    apply sound_sym_checker.
+  - unfold smt_equiv_checker in H.
+    apply sound_smt_checker.
     rewrite smt_minus_lemma.
     rewrite smt_minus_lemma.
     apply H.
-  - unfold smt_equivalence_checker in H.
+  - unfold smt_equiv_checker in H.
     apply String.eqb_eq in H.
     rewrite H.
     reflexivity.
